coq/NotInSegment.v
@@ -252,6 +252,7 @@ induction pts as [| pt₄]; intros.
   intros x y z H₁ H₂; eapply Qlt_trans; eassumption.
 Qed.
 
+(* à voir... ça dépend de ce qu'on veut...
 Lemma j_aft_prev_end :
   ∀ n pt₁ pt₂ pts ms pt₃ pts₃ ms₁ hsl₁ j αj segjk k αk segkx hsl,
   Sorted fst_lt [pt₁; pt₂ … pts]
@@ -1446,6 +1447,7 @@ destruct Hns as [Hns| Hns].
   rewrite plus_comm; simpl.
   apply eq_S; assumption.
 Qed.
+*)
 
 Lemma points_not_in_any_newton_segment₁ : ∀ pts hsl ns,
   Sorted fst_lt pts
